

## Sheet 6

### A2

2.1

$$V_{ks}(r+R) = V_{ks}(r)$$

$$\psi = u_k(r) \exp(ikr)$$

$$\left( -\frac{\hbar^2}{2m} \nabla^2 + V_{ks}(r) \right) \psi_i = E_i(r) \psi_i(r)$$

$$\left( -\frac{\hbar^2}{2m} \nabla^2 + V_{ks}(r) \right) u_{i,k} e^{-i\vec{k}\vec{r}} = E_{i,k}(r) u_{i,k}(r)$$

$$\nabla^2 u_{i,k} e^{-i\vec{k}\vec{r}} = \nabla \cdot \nabla (u_{i,k} e^{-i\vec{k}\vec{r}})$$

$$= \nabla \cdot \left( -ik u_{i,k} e^{-i\vec{k}\vec{r}} + e^{-i\vec{k}\vec{r}} \nabla u_{i,k} \right)$$

$$= \left( k^2 u_{i,k} e^{-i\vec{k}\vec{r}} + ik e^{-i\vec{k}\vec{r}} \nabla u_{i,k} + ik e^{-i\vec{k}\vec{r}} \nabla u_{i,k} + e^{-i\vec{k}\vec{r}} \nabla^2 u_{i,k} \right)$$

$$= \left( k^2 e^{-i\vec{k}\vec{r}} + 2ik e^{-i\vec{k}\vec{r}} \nabla u_{i,k} + e^{-i\vec{k}\vec{r}} \nabla^2 u_{i,k} \right)$$

$$= e^{-i\vec{k}\vec{r}} \left( k^2 + 2ik + \nabla^2 \right) u_{i,k}$$

$$= e^{-i\vec{k}\vec{r}} (k + \nabla)^2 u_{i,k}$$

$$\Rightarrow \left[ -\frac{\hbar^2}{2m} \nabla^2 + V_{ks}(r) \right] u_{i,k} e^{-i\vec{k}\vec{r}}$$

$$= -\frac{\hbar^2}{2m} e^{-i\vec{k}\vec{r}} (k + \nabla)^2 u_{i,k}(r) + V_{ks}(r) e^{-i\vec{k}\vec{r}} u_{i,k} = E_i u_{i,k} e^{-i\vec{k}\vec{r}}$$

$$\Rightarrow \left[ -\frac{\hbar^2}{2m} (k + \nabla)^2 + V_{ks} \right] u_{i,k}(r) = E_i u_{i,k}(r)$$

## A2.2

$$\psi_{ik}(r) = \sum_{\vec{G}} C_{ik,G} e^{i\vec{G}\vec{r}}$$

$$\left[ -\frac{\hbar^2}{2m} (\nabla + i\vec{k})^2 + V_{KS}(r) \right] \sum_{\vec{G}} C_{ik,G} e^{i\vec{G}\vec{r}}$$

$$(\nabla + i\vec{k})^2 e^{i\vec{G}\vec{r}} = -G^2 - 2i\vec{k}\vec{G} - k^2 = -|\vec{G} + \vec{k}|^2$$

$$\left[ \frac{\hbar^2}{2m} |\vec{G} + \vec{k}|^2 + V_{KS}(r) \right] \sum_{\vec{G}} C_{ik,G} e^{i\vec{G}\vec{r}} = E_{ik} \sum_{\vec{G}} C_{ik,G} e^{i\vec{G}\vec{r}}$$

$$\sum_{\vec{G}} \int e^{-i\vec{G}'\vec{r}} \left[ \frac{\hbar^2}{2m} |\vec{G} + \vec{k}|^2 + V_{KS}(r) \right] C_{ik,G} e^{i\vec{G}\vec{r}} d^3r = E_{ik} \sum_{\vec{G}} C_{ik,G} \int e^{i\vec{G}\vec{r}} e^{-i\vec{G}'\vec{r}} d^3r$$

$$\sum_{\vec{G}} \int e^{-i\vec{G}'\vec{r}} \left( \frac{\hbar^2}{2m} |\vec{G} + \vec{k}|^2 + V_{KS}(r) \right) C_{ik,G} e^{i\vec{G}\vec{r}} d^3r = E_{ik} \sum_{\vec{G}} C_{ik,G} \delta_{\vec{G}\vec{G}'} = \Omega E_{ik} C_{ik,\vec{G}'}$$

$$\begin{aligned} LHS &= \sum_{\vec{G}} \int e^{i(\vec{G}-\vec{G}')\vec{r}} \left( \frac{\hbar^2}{2m} |\vec{G} + \vec{k}|^2 \right) C_{ik,G} d^3r + \sum_{\vec{G}} \int e^{-i\vec{G}'\vec{r}} V_{KS}(r) C_{ik,G} e^{i\vec{G}\vec{r}} d^3r \\ &= \sum_{\vec{G}} \Omega \delta_{\vec{G}\vec{G}'} \left( \frac{\hbar^2}{2m} |\vec{G} + \vec{k}|^2 \right) C_{ik,G} + \sum_{\vec{G}} C_{ik,G} \int e^{i(\vec{G}-\vec{G}')\vec{r}} V_{KS}(r) d^3r \end{aligned}$$

$$= \sum_{\vec{G}} \Omega \delta_{\vec{G}\vec{G}'} \left( \frac{\hbar^2}{2m} |\vec{G} + \vec{k}|^2 \right) C_{ik,G} + \sum_{\vec{G}} C_{ik,G} V(\vec{G}-\vec{G}') \cdot \Omega$$

$$\Rightarrow \sum_{\vec{G}} \left[ \delta_{\vec{G}\vec{G}'} \left( \frac{\hbar^2}{2m} |\vec{G} + \vec{k}|^2 \right) + V(\vec{G}-\vec{G}') \right] C_{ik,G} = E_{ik} C_{ik,\vec{G}'}$$

$$\stackrel{\vec{G} \leftrightarrow \vec{G}'}{\rightarrow} \sum_{\vec{G}'} \left[ \delta_{\vec{G}\vec{G}'} \frac{\hbar^2}{2m} |\vec{G} + \vec{k}|^2 + V(\vec{G}' - \vec{G}) \right] C_{ik,G'} = E_{ik} C_{ik,G}$$

sollte ok sein weil  $\sum_{\vec{G}}$  über alle  $\vec{G}'$  geht